added unique id to signatures, reproved attestation and appraisal theorems

src/MonadVM.v
@@ -88,7 +88,7 @@ Definition invoke_ASP (i:ASP_ID) (l:list Arg) (tpl:Plc) (tid:TARG_ID) (x:nat) : 
 Definition encodeEv (e:EvC): BS.
 Admitted.
 
-Definition do_sig (bs:BS) (p:Plc) : BS.
+Definition do_sig (bs:BS) (p:Plc) (sigTag:BS) : BS.
 Admitted.
 
 Definition do_hash (bs:BS) (p:Plc) : BS.
@@ -110,7 +110,7 @@ Definition signEv (x:nat) : CVM EvC :=
   p <- get_pl ;;
   e <- get_ev ;;
   tag_SIG x p e ;;
-  ret (cons_gg (do_sig (encodeEv e) p) e p).
+  ret (cons_gg (do_sig (encodeEv e) p x) e p).
 
 Definition tag_HSH (x:nat) (p:Plc) (e:EvC): CVM unit :=
   add_tracem [hash x p (get_et e)].
